syntax/SLoopUnroll.v
@@ -21,6 +21,12 @@ Definition suffix_peel_unroll : nat -> SPolIRs.Loop.t -> SPolIRs.Loop.t :=
 Definition suffix_peel_unroll_changed : nat -> SPolIRs.Loop.t -> bool :=
   CoreUnroll.suffix_peel_unroll_changed.
 
+Definition block_unroll : nat -> SPolIRs.Loop.t -> SPolIRs.Loop.t :=
+  CoreUnroll.block_unroll.
+
+Definition block_unroll_changed : nat -> SPolIRs.Loop.t -> bool :=
+  CoreUnroll.block_unroll_changed.
+
 Definition peel_plan : Type :=
   CoreUnroll.peel_plan.
 
